<section xml:id="euclideanalgo">
  <title>The GCD and the Euclidean Algorithm</title>
  <definition>
    <statement>
      <p>
        Let <m>a</m> and <m>b</m> be two nonzero integers.
        A <term>common divisor</term> or
        <term>common factor</term>
        of <m>a</m> and <m>b</m> is an integer
        <m>d \in \N</m> such that <m>d</m> divides both <m>a</m> and <m>b</m>.
        The <term>greatest common divisor</term> (AKA the
        <term>highest common factor</term>) of <m>a</m> and <m>b</m> is the <term>largest</term>
        common divisor of <m>a</m> and <m>b</m>.
        We denote this integer <m>d</m> by
        <m>\gcd(a,b)</m> (you may also see the notation <m>\mathrm{hcf}(a,b)</m>.
      </p>
      <p>
        If <m>\gcd(a,b)=1</m>,
        then we say that <m>a</m> and <m>b</m> are said to be <term>coprime</term>
        or <term>relatively prime</term>.
      </p>
    </statement>
  </definition>
  <p>
    Thus <m>a</m> and <m>b</m> are coprime if and only if their only (positive) common divisor is <m>1</m>.
  </p>
  <example>
    <statement>
      <p>
        <m>\gcd(15,45)=15</m>, <m>\gcd(6,15)=3</m>, and <m>\gcd(17,91)=1</m>.
      </p>
    </statement>
  </example>
  <example>
    <statement>
      <p>
        We allow ourselves the flexibility to speak of the gcd of negative integers as well as positive ones,
        but we notice that
        <me>
          \gcd(a,b) = \gcd(a,-b) = \gcd(-a,b) = \gcd(-a,-b)
        </me>.
      </p>
      <p>
        (So for instance <m>\gcd(-6,-27) = \gcd(6, 27) = 3</m>.) As a result,
        we will mostly focus on the gcd of natural numbers.
      </p>
    </statement>
  </example>
  <p>
    For a prime <m>p>1</m> and any integer <m>n</m>, we have:
    <md>
      \gcd(p,n) = \left\{\aligned\amp 1\ \text{ if \(p\) does not divide \(n\) } ,\\ \amp p\ \text{ if \(p\)  divides \(n\) } .\\ \endaligned \right.
    </md>
  </p>
  <definition>
    <statement>
      <p>
        Let <m>a</m> and <m>b</m> be integers.
        An <term>integer linear combination</term>
        of <m>a</m> and <m>b</m> is an integer of the form <m>ma + nb</m> for some <m>m,n \in \Z</m>.
      </p>
    </statement>
  </definition>
  <p>
    Notice that a linear combination of linear combinations is a linear combination.
    That is, if <m>c</m> and <m>b</m> are each linear combinations of <m>a</m> and <m>b</m>,
    then for some integers <m>m</m>,
    <m>n</m>, <m>p</m>, and <m>q</m>,
    we have <m>c = m a + n b</m> and <m>d = p a + q b</m>.
    If we form a linear combination of <m>c</m> and <m>d</m>, we get
    <me>
      r c + s d = (rm+sp)a + (rn+sq)b
    </me>,
    which is a linear combination of <m>a</m> and <m>b</m>.
  </p>
  <p>
    A little trick that we will use repeatedly is the observation that common divisors of two integers are also divisors of linear combinations of those integers:
  </p>
  <lemma xml:id="l_easy-lemma">
    <title>Linear Combination Lemma</title>
    <statement>
      <p>
        Let <m>a</m>, <m>b</m>, and <m>d</m> be integers.
        If <m>d</m> divides both <m>a</m> and <m>b</m>,
        then <m>d</m> divides every integer linear combination of <m>a</m> and <m>b</m>.
        In other words,
        for every pair of integers <m>m,n\in\mathbb{Z}</m>,
        the integer <m>d</m> also divides <m>ma + nb</m>.
      </p>
    </statement>
  </lemma>
  <proof>
    <p>
      Since <m>d</m> divides <m>a</m> and <m>d</m> divides <m>b</m>,
      there are integers <m>s</m> and <m>t</m> so that <m>a=sd</m> and <m>b=td</m>.
      Hence
      <me>
        ma+nb=msd+ntd=(ms+nt)d
      </me>
      and so <m>d</m> divides <m>ma+nb</m>.
    </p>
  </proof>
  <example>
    <statement>
      <p>
        Let <m>a, b \in \Z</m>.
        If there is a linear combination of <m>a</m> and <m>b</m> that gives <m>1</m>,
        then <m>a</m> and <m>b</m> are coprime.
        Indeed, if <m>m,n \in \Z</m> have the property that <m>ma+nb = 1</m>,
        then any common divisor <m>d</m> of <m>a</m> and <m>b</m> must also divide <m>1</m>.
        But then <m>d=1</m>, so <m>\gcd(a,b)=1</m>.
      </p>
      <p>
        Here we'll show <m>n</m> and <m>n+1</m> are coprime: By the Linear Combination Lemma,
        <m>\gcd(n,n+1)</m> divides <m>(n+1)-n=1</m>,
        so <m>\gcd(n,n+1)</m> divides <m>1</m>.
        Thus <m>\gcd(n,n+1)=1</m>.
      </p>
    </statement>
  </example>
  <p>
    We can also use it to narrow down the gcd of two numbers:
  </p>
  <example>
    <statement>
      <p>
        For <m>n\in\mathbb{N}</m>,
        what is <m>\gcd(4n^2-2,2n)?</m> Observe that by the Linear Combination Lemma,
        <m>\gcd(4n^2-2,2n)</m> divides <m>(2n)(2n)-(4n^2-2)=2</m>,
        so the highest common factor of these numbers is either <m>1</m> or <m>2</m>.
        Since <m>2</m> divides both <m>4n^2-2</m> and <m>2n</m>,
        it also divides the <m>\gcd</m>,
        so <xref ref="l_abba">Lemma</xref>
        implies <m>\gcd(4n^2-2,2n)=2</m>.
      </p>
    </statement>
  </example>
  <p>
    How do we find the gcd for very large numbers?
    For this we use the <term>Euclidean Algorithm</term>
    which exploits the Remainder Theorem and the Linear Combination Lemma.
  </p>
  <p>
    Let <m>a,b\in\N</m>.
    Let us also assume <m>a\lt b</m>.
    We are going to construct a sequence of nonnegative integers
    <me>
      0 = r_{n+1} \lt  r_n \lt  \cdots \lt  r_2 \lt  r_1 = a \lt  r_0 = b
    </me>
    such that for each <m>k \in \N</m>, if <m>k\leq n</m>, then:
    <ol>
      <li>
        <p>
          <m>r_{k-1}</m> is an integer linear combination of <m>r_k</m> and <m>r_{k+1}</m>, and
        </p>
      </li>
      <li>
        <p>
          <m>r_{k+1}</m> is an integer linear combination of <m>r_k</m> and <m>r_{k-1}</m>.
        </p>
      </li>
    </ol>
  </p>
  <p>
    If we manage to construct a sequence with these properties,
    then <m>\gcd(a,b)</m> will be the natural number <m>r_n</m>.
    Before we perform the construction, let's understand why.
    The key is the Linear Combination Lemma.
    <ul>
      <li>
        <p>
          We first claim that <m>\gcd(a,b)</m> divides <m>r_{n}</m>.
          Note that <m>r_0=b</m> and <m>r_1=a</m> are certainly linear combinations of <m>a</m> and <m>b</m>.
          Let <m>k\in \N</m> with <m>1\leq k \leq n</m>.
          If <m>r_{k-1}</m> and <m>r_k</m> are each integer linear combinations of <m>a</m> and <m>b</m>,
          so is <m>r_{k+1}</m>.
          By induction,
          we conclude that <m>r_n</m> is a integer linear combination of <m>a</m> and <m>b</m>.
          Hence it follows from the Linear Combination Lemma<nbsp/>that <m>\gcd(a,b)</m> divides <m>r_n</m>.
        </p>
      </li>
      <li>
        <p>
          On the other hand,
          we claim that <m>r_{n}</m> divides <m>\gcd(a,b)</m>.
          This is equivalent to the claim that <m>r_n</m> is a common divisor of <m>a</m> and <m>b</m>.
          Note that since <m>r_{n+1}=0</m>,
          it follows that <m>r_{n-1}=q_{n+1}r_{n}</m> for some <m>q_{n+1}\in\Z</m>,
          so <m>r_{n}</m> divides <m>r_{n-1}</m>.
          Let <m>k\in \N</m> with <m>k \leq n</m>.
          Assume that <m>r_n</m> divides <m>r_k</m> and <m>r_{k+1}</m>;
          since <m>r_{k-1}</m> is a linear combination of <m>r_k</m> and <m>r_{k+1}</m>,
          it follows from the Linear Combination Lemma<nbsp/>that <m>r_n</m> divides <m>r_{k-1}</m> as well.
          By induction,
          we conclude that <m>r_n</m> divides <m>r_1=a</m> and <m>r_0=b</m>.
        </p>
      </li>
    </ul>
  </p>
  <p>
    This proves
    (using <xref ref="l_abba">Lemma</xref>)
    that <m>\gcd(a,b)=r_n</m>.
  </p>
  <p>
    So our goal now is to present an iterative construction of a sequence of nonnegative integers
    <me>
      0 = r_{n+1} \lt  r_n \lt  \cdots \lt  r_2 \lt  r_1 = a \lt  r_0 = b
    </me>
    such that for each <m>k \in \N</m>, if <m>k\leq n</m>, then
    <ol>
      <li>
        <p>
          <m>r_{k-1}</m> is an integer linear combination of <m>r_k</m> and <m>r_{k+1}</m>, and
        </p>
      </li>
      <li>
        <p>
          <m>r_{k+1}</m> is an integer linear combination of <m>r_k</m> and <m>r_{k-1}</m>.
        </p>
      </li>
    </ol>
  </p>
  <p>
    To begin the iteration, we set <m>r_0 = b</m> and <m>r_1 = a</m>.
    To construct the rest of the sequence,
    assume that for some <m>k\in\N</m> we have constructed nonnegative integers
    <m>r_k \lt  r_{k-1} \lt  \dots \lt  r_1 \lt  r_0</m> with the two properties above.
    Now use the Remainder Theorem to find an integers <m>q_{k+1}</m> and <m>r_{k+1}</m> such that
    <me>
      r_{k-1} = q_{k+1}r_k + r_{k+1}
    </me>.
  </p>
  <p>
    Thus <m>r_{k-1}</m> is a linear combination of <m>r_k</m> and <m>r_{k+1}</m>,
    but also <m>r_{k+1} = r_{k-1} - q_{k+1} r_k</m> so <m>r_{k+1}</m> is a linear combination of <m>r_k</m> and <m>r_{k-1}</m>.
  </p>
  <p>
    This process must terminate with <m>r_{n+1}=0</m> for some <m>n</m>,
    since the <m>r_{j}</m> are nonnegative and strictly decreasing.
    This completes the construction of the sequence
    <me>
      0 = r_{n+1} \lt  r_n \lt  \cdots \lt  r_2 \lt  r_1 = a \lt  r_0 = b
    </me>
    with the desired properties.
  </p>
  <p>
    Let's watch this algorithm in action.
  </p>
  <example>
    <statement>
      <p>
        Let <m>a = r_1 = 6</m> and <m>b = r_0 = 15</m>.
        <ul>
          <li>
            <p>
              We divide <m>15</m> by <m>6</m> to get <m>2</m> with a remainder of <m>r_2=3</m>.
            </p>
          </li>
          <li>
            <p>
              We divide <m>6</m> by <m>3</m> to get <m>2</m> with a remainder of <m>r_3 = 0</m>.
            </p>
          </li>
        </ul>
      </p>
      <p>
        Thus <m>r_2 = 3</m> is the gcd of <m>6</m> and <m>15</m>.
      </p>
    </statement>
  </example>
  <example>
    <statement>
      <p>
        Let <m>a = r_1 = 48</m> and <m>b = r_0 = 66</m>.
        <ul>
          <li>
            <p>
              We divide <m>66</m> by <m>48</m> to get <m>1</m> with a remainder of <m>r_2=18</m>.
            </p>
          </li>
          <li>
            <p>
              We divide <m>48</m> by <m>18</m> to get <m>2</m> with a remainder of <m>r_3 = 12</m>.
            </p>
          </li>
          <li>
            <p>
              We divide <m>18</m> by <m>12</m> to get <m>1</m> with a remainder of <m>r_4 = 6</m>.
            </p>
          </li>
          <li>
            <p>
              We divide <m>12</m> by <m>6</m> to get <m>2</m> with a remainder of <m>r_5 = 0</m>.
            </p>
          </li>
        </ul>
      </p>
      <p>
        Thus <m>r_4 = 6</m> is the gcd of <m>48</m> and <m>66</m>.
      </p>
    </statement>
  </example>
  <example>
    <statement>
      <p>
        Let <m>a = r_1 = 120</m> and <m>b = r_0 = 214</m>.
        <ul>
          <li>
            <p>
              We divide <m>214</m> by <m>120</m> to get <m>1</m> with a remainder of <m>r_2=94</m>.
            </p>
          </li>
          <li>
            <p>
              We divide <m>120</m> by <m>94</m> to get <m>1</m> with a remainder of <m>r_3 = 26</m>.
            </p>
          </li>
          <li>
            <p>
              We divide <m>94</m> by <m>26</m> to get <m>3</m> with a remainder of <m>r_4 = 16</m>.
            </p>
          </li>
          <li>
            <p>
              We divide <m>26</m> by <m>16</m> to get <m>1</m> with a remainder of <m>r_5 = 10</m>.
            </p>
          </li>
          <li>
            <p>
              We divide <m>16</m> by <m>10</m> to get <m>1</m> with a remainder of <m>r_6 = 6</m>.
            </p>
          </li>
          <li>
            <p>
              We divide <m>10</m> by <m>6</m> to get <m>1</m> with a remainder of <m>r_7 = 4</m>.
            </p>
          </li>
          <li>
            <p>
              We divide <m>6</m> by <m>4</m> to get <m>1</m> with a remainder of <m>r_8 = 2</m>.
            </p>
          </li>
          <li>
            <p>
              We divide <m>4</m> by <m>2</m> to get <m>2</m> with a remainder of <m>r_9 = 0</m>.
            </p>
          </li>
        </ul>
      </p>
      <p>
        Thus <m>r_8 = 2</m> is the gcd of <m>120</m> and <m>214</m>.
      </p>
    </statement>
  </example>
  <example>
    <statement>
      <p>
        Let <m>a = r_1 = 14</m> and <m>b = r_0 = 348</m>.
        <ul>
          <li>
            <p>
              We divide <m>348</m> by <m>14</m> to get <m>24</m> with a remainder of <m>r_2=12</m>.
            </p>
          </li>
          <li>
            <p>
              We divide <m>14</m> by <m>12</m> to get <m>1</m> with a remainder of <m>r_3 = 2</m>.
            </p>
          </li>
          <li>
            <p>
              We divide <m>12</m> by <m>2</m> to get <m>6</m> with a remainder of <m>r_4 = 0</m>.
            </p>
          </li>
        </ul>
      </p>
      <p>
        Thus <m>r_3 = 2</m> is the gcd of <m>14</m> and <m>348</m>.
      </p>
    </statement>
  </example>
  <example>
    <statement>
      <p>
        Let <m>a = r_1 = 2059</m> and <m>b = r_0 = 6744</m>.
        <ul>
          <li>
            <p>
              We divide <m>6744</m> by <m>2059</m> to get <m>3</m> with a remainder of <m>r_2=567</m>.
            </p>
          </li>
          <li>
            <p>
              We divide <m>2059</m> by <m>567</m> to get <m>3</m> with a remainder of <m>r_3 = 358</m>.
            </p>
          </li>
          <li>
            <p>
              We divide <m>567</m> by <m>358</m> to get <m>1</m> with a remainder of <m>r_4 = 209</m>.
            </p>
          </li>
          <li>
            <p>
              We divide <m>358</m> by <m>209</m> to get <m>1</m> with a remainder of <m>r_5 = 149</m>.
            </p>
          </li>
          <li>
            <p>
              We divide <m>209</m> by <m>149</m> to get <m>1</m> with a remainder of <m>r_6 = 60</m>.
            </p>
          </li>
          <li>
            <p>
              We divide <m>149</m> by <m>60</m> to get <m>2</m> with a remainder of <m>r_7 = 29</m>.
            </p>
          </li>
          <li>
            <p>
              We divide <m>60</m> by <m>29</m> to get <m>2</m> with a remainder of <m>r_8 = 2</m>.
            </p>
          </li>
          <li>
            <p>
              We divide <m>29</m> by <m>2</m> to get <m>14</m> with a remainder of <m>r_9 = 1</m>.
            </p>
          </li>
          <li>
            <p>
              We divide <m>2</m> by <m>1</m> to get <m>2</m> with a remainder of <m>r_{10} = 0</m>.
            </p>
          </li>
        </ul>
      </p>
      <p>
        Thus <m>r_9 = 1</m> is the gcd of <m>2059</m> and <m>6744</m>.
        In particular, <m>2059</m> and <m>6744</m> are coprime.
      </p>
    </statement>
  </example>
  <p>
    One important corollary of the Euclidean Algorithm is the following.
  </p>
  <theorem xml:id="t_lincombgcd">
    <title>Bezout’s  Identity</title>
    <statement>
      <p>
        Let <m>a</m> and <m>b</m> be integers.
        Then <m>\gcd(a,b)</m> is an integer linear combination of <m>a</m> and <m>b</m>.
        That is, there are integers <m>s</m> and <m>t</m> so that <m>\gcd(a,b)=sa+tb</m>.
      </p>
    </statement>
  </theorem>
  <p>
    Let's revisit some of the examples above to find the <m>s</m> and <m>t</m>.
  </p>
  <example>
    <statement>
      <p>
        Let <m>a = r_1 = 6</m> and <m>b = r_0 = 15</m>.
        <ul>
          <li>
            <p>
              We divide <m>15</m> by <m>6</m> to get <m>2</m> with a remainder of <m>r_2=3</m>.
            </p>
          </li>
          <li>
            <p>
              We divide <m>6</m> by <m>3</m> to get <m>2</m> with a remainder of <m>r_3 = 0</m>.
            </p>
          </li>
        </ul>
      </p>
      <p>
        Thus <m>\gcd(6,15) = 3 = 15-2\cdot 6</m>.
      </p>
    </statement>
  </example>
  <example>
    <statement>
      <p>
        Let <m>a = r_1 = 48</m> and <m>b = r_0 = 66</m>.
        <ul>
          <li>
            <p>
              We divide <m>66</m> by <m>48</m> to get <m>1</m> with a remainder of <m>r_2=18</m>.
            </p>
          </li>
          <li>
            <p>
              We divide <m>48</m> by <m>18</m> to get <m>2</m> with a remainder of <m>r_3 = 12</m>.
            </p>
          </li>
          <li>
            <p>
              We divide <m>18</m> by <m>12</m> to get <m>1</m> with a remainder of <m>r_4 = 6</m>.
            </p>
          </li>
          <li>
            <p>
              We divide <m>12</m> by <m>6</m> to get <m>2</m> with a remainder of <m>r_5 = 0</m>.
            </p>
          </li>
        </ul>
      </p>
      <p>
        Thus <m>\gcd(48,66) = 6 = 18-12 = 3\cdot 18-48 = 3\cdot 66 -4\cdot 48</m>.
      </p>
    </statement>
  </example>
  <example>
    <statement>
      <p>
        Let <m>a = r_1 = 2059</m> and <m>b = r_0 = 6744</m>.
        <ul>
          <li>
            <p>
              We divide <m>6744</m> by <m>2059</m> to get <m>3</m> with a remainder of <m>r_2=567</m>.
            </p>
          </li>
          <li>
            <p>
              We divide <m>2059</m> by <m>567</m> to get <m>3</m> with a remainder of <m>r_3 = 358</m>.
            </p>
          </li>
          <li>
            <p>
              We divide <m>567</m> by <m>358</m> to get <m>1</m> with a remainder of <m>r_4 = 209</m>.
            </p>
          </li>
          <li>
            <p>
              We divide <m>358</m> by <m>209</m> to get <m>1</m> with a remainder of <m>r_5 = 149</m>.
            </p>
          </li>
          <li>
            <p>
              We divide <m>209</m> by <m>149</m> to get <m>1</m> with a remainder of <m>r_6 = 60</m>.
            </p>
          </li>
          <li>
            <p>
              We divide <m>149</m> by <m>60</m> to get <m>2</m> with a remainder of <m>r_7 = 29</m>.
            </p>
          </li>
          <li>
            <p>
              We divide <m>60</m> by <m>29</m> to get <m>2</m> with a remainder of <m>r_8 = 2</m>.
            </p>
          </li>
          <li>
            <p>
              We divide <m>29</m> by <m>2</m> to get <m>14</m> with a remainder of <m>r_9 = 1</m>.
            </p>
          </li>
          <li>
            <p>
              We divide <m>2</m> by <m>1</m> to get <m>2</m> with a remainder of <m>r_{10} = 0</m>.
            </p>
          </li>
        </ul>
      </p>
      <p>
        Thus
        <md>
          <mrow>\gcd(6744, 2059) = 1 \amp = 29 - 14\cdot 2</mrow>
          <mrow>\amp = 29\cdot 29 - 14 \cdot 60</mrow>
          <mrow>\amp = 29\cdot 149-72\cdot 60</mrow>
          <mrow>\amp = 101\cdot 149-72\cdot 209</mrow>
          <mrow>\amp = 101\cdot 358-173\cdot 209</mrow>
          <mrow>\amp = 274\cdot 358-173\cdot 567</mrow>
          <mrow>\amp = 274\cdot 2059-995\cdot 567</mrow>
          <mrow>\amp = 3259\cdot 2059-995\cdot 6744</mrow>
        </md>
      </p>
    </statement>
  </example>
  <p>
    Bezout's Identity is incredibly useful,
    even in examples that seem to have nothing to do with the gcd:
  </p>
  <exercise>
    <statement>
      <p>
        Let <m>a</m> and <m>b</m> be coprime integers.
        Show that
        <ul>
          <li>
            <title>(i)</title>
            <p>
              If <m>a</m> divides <m>c</m> and <m>b</m> divides <m>c</m> then <m>ab</m> divides <m>c</m>.
            </p>
          </li>
          <li>
            <title>(ii)</title>
            <p>
              If <m>a</m> divides <m>bc</m> then <m>a</m> divides <m>c</m>.
            </p>
          </li>
        </ul>
      </p>
      <p>
        Show that both parts of this result can fail if <m>a</m> and <m>b</m> are not coprime.
      </p>
    </statement>
    <solution>
      <ul>
        <li>
          <title>(i)</title>
          <p>
            Since <m>a</m> and <m>b</m> are coprime,
            we can find integers <m>s</m> and <m>t</m> so that <m>sa + tb = 1</m>.
            If <m>a</m> divides <m>c</m> then we can write <m>c = ax</m>,
            and if <m>b</m> divides <m>c</m> then we can write <m>c = by</m> for some <m>x,y \in \Z</m>.
            Then <m>c = csa + ctb = (by)sa + (ax)tb = (ab)sy + (ab)xt</m>,
            so <m>ab</m> divides <m>c</m>.
          </p>
        </li>
        <li>
          <title>(ii)</title>
          <p>
            As in (i), <m>c = csa + ctb</m>.
            If <m>a</m> divides <m>bc</m> then write <m>az = bc</m> for some integer <m>z</m>,
            and then we have <m>c = csa + t(az) = a(cs + tz)</m>,
            so <m>a</m> divides <m>c</m>.
          </p>
        </li>
      </ul>
    </solution>
  </exercise>
  <exercise>
    <p>
      Show that if <m>a, b</m> are postive integers,
      and <m>d=gcd(a,b)</m> then there exist positive integers
      <m>s,
      t</m> such that <m>d=sa-tb</m>.
      <em>Note:</em> that this exercise differs from Bezout’s Identity,
      in that we ask <m>s, t</m> to be <em>positive</em>.
    </p>
    <solution>
      <p>
        <em>Claim</em>: If <m>a,b</m> are positive integers and <m>d=gcd(a,b)</m>,
        we can find positive integers
        <m>s,
        t \in\mathbb{Z}</m> such that <m>d=sa-tb</m>.
      </p>
      <proof>
      <p>
        By the Euclidean algorithm,
        we can find integers <m>s,t\in\mathbb{Z}</m>, such that
        <men xml:id="gcdeqn">
          d=sa+tb
        </men>
      </p>
      <p>
        Since <m>0\lt d\leq a,b</m>,
        at most one of <m>s</m> and <m>t</m> can be positive,
        and at most one can be non-positive (i.e. zero or negative).
        If it happens that <m>t</m> is negative,
        then we will have produced the desired expression for <m>d</m> (by writing <m>d=sa - (-t)b</m>).
      </p>
      <p>
        In case <m>t</m> is non-negative,
        we can apply the following observation:
      </p>
      <lemma>
        <statement>
          <p>
            The integers <m>s</m> and <m>t</m> satisfy Equation <xref ref="gcdeqn"/> if,
            and only if,
            the integers <m>s+kb</m> and <m>t-ka</m> do as well, for any integer <m>k</m>.
          </p>
        </statement>
      </lemma>
      <proof>
        <p>
          We have <m>(s+kb)a + (t-ka)b = sa+tb</m>,
          simply by expanding the LHS, so one finds the same condition for both pairs.
        </p>
      </proof>
      <p>
        Choosing <m>k</m> sufficiently large,
        we can replace <m>t</m> by <m>t-ka</m> so that it is negative.
        It follows then that <m>s+kb</m> is positive.
      </p>
      </proof>
    </solution>
  </exercise>
</section>