<section xml:id="inductionsection">
  <title>Induction</title>
  <p>
    The main topic of this chapter is the following fundamental property of the natural numbers/axiom of mathematics called the Principle of Mathematical Induction.
  </p>
  <definition>
    <title>The Principle of Mathematical Induction</title>
    <statement>
      <p>
        Given a list of statements
        <m>P(k),P(k+1),..</m>., we may conclude that <m>P(n)</m> is true for every integer <m>n\geqslant k</m>
        <term>provided that</term>
        <ul>
          <li>
            <p>
              we know that <m>P(k)</m> is true (base case)
            </p>
          </li>
          <li>
            <p>
              and we can prove that <m>P(n)\Rightarrow P(n+1)</m> for any integer <m>n\geqslant k</m>
              (induction step).
            </p>
          </li>
        </ul>
      </p>
    </statement>
  </definition>
  <p>
    The basic idea of an induction proof is to proceed step by step.
    We prove the base case is true,
    and the induction step retains truth as we move from <m>P(n)</m> to <m>P(n+1)</m>.
  </p>
  <p>
    A full written proof by induction has the following four parts clearly separated.
    <ol>
      <li>
        <p>
          A clear and explicit statement of the
          <q>induction hypothesis</q>
          <m>P(n)</m> and the intention to prove by induction.
        </p>
      </li>
      <li>
        <p>
          Prove a
          <q>base case</q>
          is true.
          Typically prove the single statement <m>P(1)</m>.
        </p>
      </li>
      <li>
        <p>
          Prove the
          <q>induction step</q>. Typically,
          if <m>P(n)</m> is true then <m>P(n+1)</m> is also true.
        </p>
      </li>
      <li>
        <p>
          Conclude that steps (2) and (3) allow the conclusion that <m>P(n)</m> is true for all natural numbers <m>n</m> by the principal of mathematical induction.
        </p>
      </li>
    </ol>
  </p>
  <p>
    Mathematics written for experts might skimp on some of the detail,
    e.g. saying
    <q>the base case is trivial</q>. In this course your proofs must be written systematically using all four parts of the format described above.
  </p>
  <example>
    <statement>
      <p>
        For <m>n\in\mathbb{N}</m>, <m>\sum_{k=1}^{n}k=\frac{n(n+1)}{2}</m>.
      </p>
    </statement>
    <proof>
      <p>
        Let <m>P(n)</m> be the statement that <m>\sum_{k=1}^{n}k=\frac{n(n+1)}{2}</m>.
        We prove that <m>P(n)</m> is true for all
        <m>n\in\mathbb{N}</m> by induction as follows:
        <ul>
          <li>
            <p>
              <em>Base Case:</em> First let's prove <m>P(1)</m>.
              This is just
              <me>
                \sum_{k=1}^{1}k=1=\frac{1(1+1)}{2}
              </me>.
              Thus, the base case is true.
            </p>
          </li>
          <li>
            <p>
              <em>Induction Step:</em> Assume <m>P(n)</m> holds and consider
              <me>
                \sum_{k=1}^{n+1}k =\left({\color{magenta} \sum_{k=1}^{n} k}\right) + (n+1)  = {\color{magenta} \frac{n(n+1)}{2}} +(n+1) = \frac{(n+1)(n+2)}{2}
              </me>.
              where we used the statement <m>P(n)</m> to replace
              <m>\sum_{k=1}^{n} k</m> with <m>\frac{n(n+1)}{2}</m>.
              Hence <m>\sum_{k=1}^{n+1}k=\frac{(n+1)(n+2)}{2}</m> which proves that <m>P(n)\Rightarrow P(n+1)</m> is true.
            </p>
          </li>
        </ul>
      </p>
      <p>
        Since we have shown the base case and induction step,
        <m>P(n)</m> is true for all <m>n</m> by induction.
      </p>
    </proof>
  </example>
  <exercise>
    <statement>
      <p>
        Prove the following formulas by induction:
        <ol label="labelalph">
          <li>
            <p>
              <m>\sum_{k=1}^{n} k^{2} = \frac{n(n+1)(2n+1)}{6}</m>.
            </p>
          </li>
          <li>
            <p>
              <m>\sum_{k=1}^{n} k^{3} = \left(\frac{n(n+1)}{2}\right)^{2}</m>.
            </p>
          </li>
        </ol>
      </p>
      <p>
        It turns out that for all powers <m>p</m> there is a degree <m>p+1</m> polynomial that gives a formula for the value of <m>\sum_{k=1}^{n} k^{p}</m>.
        To learn more, read up on <term>Bernoulli numbers</term>.
      </p>
    </statement>
  </exercise>
  <p>
    Some statements may not be true for all <m>n\geq 1</m> but maybe for <m>n\geq k</m> for some <m>k</m>,
    and depending on the problem you will need to figure out what this <m>k</m> is.
  </p>
  <example>
    <statement>
      <p>
        For which <m>n\in\mathbb{N}</m> do we have <m>2^{n}\lt n!</m>?
        If we plug in <m>n=1,2,3</m> this inequality fails,
        but for <m>n\geq 4</m> it starts to hold.
        This gives rise to the following conjecture:
      </p>
      <p>
        <em>Claim:</em> <m>2^{n}\lt n!</m> for <m>n\geq 4</m>.
      </p>
    </statement>
    <proof>
      <p>
        We prove by induction.
        Let <m>P(n)</m> be the statement that <m>2^{n}\lt n!</m>.
        <ul>
          <li>
            <p>
              <em>Base case:</em> The base case is <m>n=4</m>,
              and it holds because <m>2^{4} = 16 \lt 4!=24</m>.
            </p>
          </li>
          <li>
            <p>
              <em>Induction Step:</em> Assume <m>P(n)</m> is true,
              i.e. {<m>2^{n}\lt n!</m>} for some <m>n\geq 4</m>, then
              <me>
                2^{n+1} = {\color{magenta} 2^{n}}\cdot 2 \lt  {\color{magenta}n!}\cdot 2 \lt  n! \cdot (n+1)=(n+1)!
              </me>.
            </p>
          </li>
        </ul>
      </p>
      <p>
        Since we have shown the base case and induction step,
        <m>P(n)</m> is true for all <m>n\geq 4</m> by induction.
      </p>
    </proof>
  </example>
  <p>
    Some problems can be proven with or without induction:
  </p>
  <exercise>
    <statement>
      <p>
        Prove that <m>n^{3}-n</m> is divisible by <m>6</m> for all <m>n\in\mathbb{N}</m>,
        first by induction, then without induction.
      </p>
    </statement>
  </exercise>
  <p>
    The following formula will be very useful throughout this course:
  </p>
  <theorem>
    <title>Geometric Series Formula</title>
    <statement>
      <p>
        Let <m>x\neq 1</m> be a real number.
        Then for <m>N\in\mathbb{N}</m>,
        <men xml:id="e_gs">
          \sum_{n=1}^{N} x^{n}=\frac{x-x^{N+1}}{1-x} \;\;\;and \;\;\;  \sum_{n=0}^{N} x^{n}=\frac{1-x^{N+1}}{1-x}
        </men>
      </p>
    </statement>
  </theorem>
  <proof>
    <p>
      The second equation follows from the first
      (just by adding <m>1</m>),
      so we just need to prove the first.
      We prove this by induction.
      <ul>
        <li>
          <p>
            <em>Base case:</em> If <m>N=1</m>, then
            <me>
              \frac{x-x^{2}}{1-x} = \frac{x(1-x)}{1-x}=x=\sum_{n=1}^{1} x^{n}
            </me>.
          </p>
        </li>
        <li>
          <p>
            <em>Induction Step:</em> Suppose <xref ref="e_gs"/> holds for some <m>N</m>.
            Then
            <me>
              \sum_{n=1}^{N+1} x^{n} =x^{N+1}+ \sum_{n=1}^{N} x^{n} =x^{N+1} + \frac{x-x^{N+1}}{1-x} =\frac{x^{N+1}-x^{N+2}}{1-x} + \frac{x-x^{N+1}}{1-x} =\frac{x-x^{N+2}}{1-x}
            </me>.
            This proves the induction step.
            Thus, <xref ref="e_gs"/> holds for all <m>N\in\mathbb{N}</m> by induction.
          </p>
        </li>
      </ul>
    </p>
  </proof>
</section>