<section xml:id="logicalequivalence">
  <title>Logical equivalence</title>
  <p>
    This idea of
    <q>repackaging</q>
    a sentence in another way is called
    <term>logical equivalence</term>.
  </p>
  <definition>
    <statement>
      <p>
        We say that two statements <m>A</m> and <m>B</m> are <term>equivalent</term>
        if <m>A</m> is true if and only if <m>B</m> is true.
      </p>
    </statement>
  </definition>
  <p>
    One also says
    <q><m>A</m> if and only if <m>B</m></q>
    or
    <q><m>A</m> iff <m>B</m></q>
    or <m>A \iff B</m>.
    Here is the truth table for this connective:
  </p>
  <tabular>
    <row>
      <cell><m>A</m></cell>
      <cell><m>B</m></cell>
      <cell><m>A \iff B</m></cell>
    </row>
    <row bottom="minor">
      <cell></cell>
      <cell></cell>
      <cell></cell>
    </row>
    <row>
      <cell>T</cell>
      <cell>T</cell>
      <cell>T</cell>
    </row>
    <row>
      <cell>T</cell>
      <cell>F</cell>
      <cell>F</cell>
    </row>
    <row>
      <cell>F</cell>
      <cell>T</cell>
      <cell>F</cell>
    </row>
    <row>
      <cell>F</cell>
      <cell>F</cell>
      <cell>T</cell>
    </row>
  </tabular>
  <p>
    In other words,
    <m>A \iff B</m> is the same statement as <m>(A\implies B) \wedge (B \implies A)</m>.
  </p>
  <p>
    Equivalence behaves like
    <q>=</q>
    does in algebra:
    you are free to swap one statement for another equivalent statement.
    For example, if <m>A\iff B</m>,
    then the statement <m>A \vee C</m> is equivalent to the statement <m>B \vee C</m>.
  </p>
  <example>
    <statement>
      <p>
        Let <m>A</m> be a statement.
        The <term>double negation</term> of <m>A</m> is the statement <m>\overline{\overline{A}}</m>.
        Then <m>\overline{\overline{A}}</m> is equivalent to <m>A</m>.
        In other words, <m>\overline{\overline{A}} \iff A</m>.
        Indeed, <m>A</m> is true if and only if <m>\overline{A}</m> is false,
        which happens if and only if <m>\overline{\overline{A}}</m> is true.
      </p>
    </statement>
  </example>
  <p>
    To prove <m>A\iff B</m>,
    you'll usually have to prove <term>both</term>
    <m>A\implies B</m> and <m>B\implies A</m>.
  </p>
  <theorem>
    <statement>
      <p>
        Let <m>A</m> and <m>B</m> be statements.
        Then <m>A \implies B</m> is equivalent to <m>\overline{A} \vee B</m>.
        That is, <m>(A \implies B) \iff (\overline{A} \vee B)</m>.
      </p>
    </statement>
  </theorem>
  <proof>
    <p>
      We begin with the forward direction;
      that is, we shall show first that <m>(A \implies B) \implies (\overline{A} \vee B)</m>.
      So assume <m>A\implies B</m>.
      We aim to show <m>\overline{A} \vee B</m>.
    </p>
    <p>
      There are two options for <m>A</m>:
      it is either true or false.
      Let's consider these options in turn:
      <ul>
        <li>
          <p>
            If <m>A</m> is false, then <m>\overline{A}</m> is true,
            and so certainly <m>\overline{A} \vee B</m> is true as well.
          </p>
        </li>
        <li>
          <p>
            If <m>A</m> is true, then since we are assuming
            <m>A\implies B</m>, we can conclude <m>B</m>.
            Thus <m>\overline{A} \vee B</m> is true as well.
          </p>
        </li>
      </ul>
    </p>
    <p>
      Either way, we see that <m>\overline{A} \vee B</m> holds,
      so it follows that <m>A\implies B</m> implies <m>\overline{A} \vee B</m>.
    </p>
    <p>
      Now we prove the reverse direction;
      that is, we shall show that <m>(\overline{A} \vee B) \implies (A \implies B)</m>.
      Assume <m>\overline{A} \vee B</m>.
      We aim to show that <m>A\Rightarrow B</m> is true.
      To prove this, we assume that <m>A</m> is true,
      and we aim to conclude <m>B</m>.
      But we are <term>assuming</term> that either
      <m>\overline{A}</m> is true or <m>B</m> is true.
      Since <m>A</m> is true, <m>\overline{A}</m> is false.
      So <m>B</m> must be true.
      Thus, we conclude <m>A\implies B</m>,
      and so we have shown that <m>\overline{A} \vee B</m> implies <m>A \implies B</m>.
    </p>
  </proof>
  <theorem>
    <statement>
      <p>
        Let <m>A</m> and <m>B</m> be statements.
        Then <m>A \implies B</m> is equivalent to <m>\overline{B} \implies \overline{A}</m>.
        That is, <m>(A \implies B) \iff (\overline{A} \vee B)</m>.
      </p>
    </statement>
  </theorem>
  <proof>
    <p>
      We begin with the forward direction;
      that is, we shall show first that <m>(A \implies B) \implies (\overline{B} \implies \overline{A})</m>.
      So assume <m>A\implies B</m>.
      We aim to show that <m>\overline{B} \implies \overline{A}</m>.
      So assume <m>\overline{B}</m>;
      that is, that <m>B</m> is false.
    </p>
    <p>
      The previous theorem shows that
      <m>A \implies B</m> is equivalent to <m>\overline{A} \vee B</m>.
      Since <m>B</m> is false,
      the only remaining option is that <m>\overline{A}</m> holds.
      We have thus shown that <m>\overline{B} \implies \overline{A}</m>.
    </p>
    <p>
      Now we prove the reverse direction;
      that is, we shall show that <m>(\overline{B} \implies \overline{A}) \implies (A \implies B)</m>.
      So assume that <m>\overline{B} \implies \overline{A}</m>.
      We aim to show that <m>A \implies B</m>.
      So assume <m>A</m>.
      We aim to deduce <m>B</m>.
    </p>
    <p>
      By the previous theorem,
      <m>\overline{B} \implies \overline{A}</m> is equivalent to <m>\overline{\overline{B}} \vee \overline{A}</m>,
      which is in turn equivalent to <m>B \vee \overline{A}</m>.
      Since <m>A</m> is true, <m>\overline{A}</m> is false,
      and so the only option remaining is that <m>B</m> holds.
      Thus we have shown that <m>A \implies B</m>.
    </p>
  </proof>
</section>