<section xml:id="logicexercises">
  <title>Exercises</title>
  <p>
    The relevant exercises in Liebeck's book are at the end of Chapter 1.
  </p>
  <exercise>
    <statement>
      <p>
        Find statements <m>A</m> and <m>B</m> so that <m>A\Rightarrow B</m> is true but
        <ol label="labelalph">
          <li>
            <p>
              <m>A</m> is false and <m>B</m> is true.
            </p>
          </li>
          <li>
            <p>
              <m>B</m> is false.
            </p>
          </li>
        </ol>
      </p>
    </statement>
    <solution>
      <p>
        <ol label="labelalph">
          <li>
            <p>
              Recall that <m>A\Rightarrow B</m> is equivalent to <m>\bar{A}</m> or <m>B</m>,
              so we just need to find a statement so that <m>A</m> is false
              (so <m>\bar{A}</m> is true)
              and <m>B</m> is true.
              This could be <m>A</m>=
              <q>2 is odd</q>
              and <m>B</m>=
              <q>2 is even.</q>
            </p>
          </li>
          <li>
            <p>
              Recall that <m>A\Rightarrow B</m> is equivalent to <m>\bar{A}</m> or <m>B</m>,
              so if <m>B</m> is false, then <m>\bar{A}</m> must be true (i.e.
              <m>A</m> is false).
              We can let <m>A=B</m>=
              <q>2 is odd</q>, for example.
            </p>
          </li>
        </ol>
      </p>
    </solution>
  </exercise>
  <exercise>
    <statement>
      <p>
        Show that <m>A\Rightarrow B</m> is not equivalent to <m>A\Leftarrow B</m>,
        either by finding examples or using their truth tables.
      </p>
    </statement>
    <solution>
      <p>
        One could have A=
        <q><m>n</m> is a prime bigger than 2</q>
        and B=
        <q><m>n</m> is odd.</q>
      </p>
      <p>
        Recall that <m>A\Rightarrow B</m> is equivalent to
        <q><m>\bar{A}</m> or <m>B</m>,</q>
        and <m>B\Rightarrow A</m> is equivalent to
        <q><m>\bar{B}</m> or <m>A</m>,</q>
        which have truth tables
      </p>
      <tabular>
        <row>
          <cell><m>A</m></cell>
          <cell><m>B</m></cell>
          <cell><m>\bar{A}</m></cell>
          <cell><m>\bar{A}</m> or <m>{B}</m></cell>
        </row>
        <row bottom="minor">
          <cell></cell>
          <cell></cell>
          <cell></cell>
          <cell></cell>
        </row>
        <row>
          <cell>T</cell>
          <cell>T</cell>
          <cell>F</cell>
          <cell>T</cell>
        </row>
        <row>
          <cell>T</cell>
          <cell>F</cell>
          <cell>F</cell>
          <cell>F</cell>
        </row>
        <row>
          <cell>F</cell>
          <cell>T</cell>
          <cell>T</cell>
          <cell>T</cell>
        </row>
        <row>
          <cell>F</cell>
          <cell>F</cell>
          <cell>T</cell>
          <cell>T</cell>
        </row>
      </tabular>
      <tabular>
        <row>
          <cell><m>A</m></cell>
          <cell><m>B</m></cell>
          <cell><m>\bar{B}</m></cell>
          <cell><m>\bar{B}</m> or <m>{A}</m></cell>
        </row>
        <row bottom="minor">
          <cell></cell>
          <cell></cell>
          <cell></cell>
          <cell></cell>
        </row>
        <row>
          <cell>T</cell>
          <cell>T</cell>
          <cell>F</cell>
          <cell>T</cell>
        </row>
        <row>
          <cell>T</cell>
          <cell>F</cell>
          <cell>F</cell>
          <cell>T</cell>
        </row>
        <row>
          <cell>F</cell>
          <cell>T</cell>
          <cell>T</cell>
          <cell>T</cell>
        </row>
        <row>
          <cell>F</cell>
          <cell>F</cell>
          <cell>T</cell>
          <cell>F</cell>
        </row>
      </tabular>
      <p>
        Since the truth tables are not the same, they are not equivalent.
      </p>
    </solution>
  </exercise>
  <exercise>
    <statement>
      <p>
        Suppose <m>A,B,C</m> are statements.
        Negate the statements
        <me>
          A\mbox{ and } (B \mbox{ or } C)
        </me>
        and
        <me>
          A\mbox{ or } (B \mbox{ and } C)
        </me>.
      </p>
    </statement>
    <solution>
      <p>
        The negations are, respectively,
        <me>
          \bar{A} \mbox{ or }  (\bar{B}\mbox{ and } \bar{C})
        </me>
        and
        <me>
          \bar{A} \mbox{ and }  (\bar{B}\mbox{ or } \bar{C})
        </me>.
      </p>
    </solution>
  </exercise>
  <exercise>
    <statement>
      <p>
        Suppose <m>P,Q,R</m> are statements and <m>P\Rightarrow Q</m>,
        <m>Q\Rightarrow R</m> and <m>R\Rightarrow P</m>.
        Show that <m>P\Leftrightarrow R</m>.
      </p>
    </statement>
    <solution>
      <p>
        Assume <m>P\Rightarrow Q</m>,
        <m>Q\Rightarrow R</m> and <m>R\Rightarrow P</m>,
        we will show that <m>P\Leftrightarrow R</m>.
        To prove this, we need to show
        <m>P\Rightarrow R</m> and <m>R\Rightarrow P</m>.
        We area already assuming <m>R\Rightarrow P</m>,
        so we just need to prove <m>P\Rightarrow R</m>.
        Hence, assume <m>P</m>.
        Then since <m>P\Rightarrow Q</m>,
        we know <m>Q</m> is also true,
        and since <m>Q\Rightarrow R</m>,
        we also know <m>R</m> is true.
        Thus <m>P\Rightarrow R</m>.
      </p>
    </solution>
  </exercise>
  <exercise>
    <statement>
      <p>
        Negate the following statements
        <ol label="labelalph">
          <li>
            <p>
              <m>(\forall x \;\; P)\Rightarrow ((\exists y \mbox{ s.t. } Q) \mbox { and }R)</m>.
            </p>
          </li>
          <li>
            <p>
              <m>\forall x\;\; \exists y \mbox{ s.t. } P\Rightarrow Q</m>
            </p>
          </li>
          <li>
            <p>
              <m>\exists x \mbox{ s.t. } ((\forall y \;\; A)\Rightarrow (\exists z \mbox{ s.t. } B))</m>.
            </p>
          </li>
        </ol>
      </p>
    </statement>
    <solution>
      <p>
        <ol label="labelalph">
          <li>
            <p>
              <m>(\forall x \;\; P) \mbox{ and } ((\forall y \;\; \bar{Q}) \mbox { or }\bar{R})</m>.
            </p>
          </li>
          <li>
            <p>
              <m>\exists x \mbox{ s.t. } \;\; \forall y \; (P\mbox{ and } \bar{Q})</m>.
            </p>
          </li>
          <li>
            <p>
              <m>\forall x ( (\forall y \;\; A) \mbox{ and } (\forall z \bar{B}))</m>.
            </p>
          </li>
        </ol>
      </p>
    </solution>
  </exercise>
</section>