<section xml:id="polynomialsexercises">
  <title>Exercises</title>
  <exercise>
    <statement>
      <p>
        Find the (complex) roots of the following polynomials:
      </p>
      <p>
        (a) <m>x^2-5x+7-i=0</m>.
      </p>
    </statement>
    <solution>
      <p>
        Recall that the roots of this polynomial are
        <me>
          x= \frac{5\pm z}{2}
        </me>
        where <m>z</m> are the solutions to
        <me>
          z^2 = 5^2-4\cdot (7-i)\cdot 1  = 25-28+4i = -3+4i
        </me>.
      </p>
      <p>
        If we set <m>z=a+ib</m>, this gives
        <me>
          a^2-b^2+2abi = -3+4i
        </me>.
      </p>
      <p>
        So in particular, <m>2ai = 4i</m> and <m>a^2-b^2 = -3</m>.
        Moreover,
        <me>
          |z^2|= |-3 + 4i| = 5
        </me>
      </p>
      <p>
        Thus,
        <me>
          5=|z^2|=|z|^2 = \sqrt{a^2+b^2}^2 = a^2+b^2
        </me>
      </p>
      <p>
        Adding this to <m>a^2-b^2=-3</m> implies <m>2a^2 = 2</m>,
        so <m>a^2=1</m>, and so <m>a = \pm 1</m>.
        Similarly, subtracting <m>a^2-b^2=-3</m> from the above equation gives <m>2b^2 = 8</m>,
        so <m>b=\pm 2</m>.
        Finally, <m>2ab = 4</m> implies that <m>a</m> and <m>b</m> have the same algebraic sign,
        so we must have <m>a+ib</m> is <m>1+2i</m> or <m>-1-2i</m> as our two solutions for <m>z</m>.
        Hence,
        <me>
          x=\frac{5 \pm (1+2i)}{2}
        </me>
        so <m>x</m> is either <m>3+i</m> or <m>2-i</m>.
      </p>
      <p>
        We can substitute these in to check, e.g. (just the first)
        <me>
          (3+i)^2-5(3+i)+7-i = (8+6i)-5(3+i)+7-i =0
        </me>
      </p>
    </solution>
    <p>
      (b) <m>x^4 -x^2 - 1 = 0</m>.
    </p>
    <solution>
      <p>
        Let <m>y=x^2</m>.
        Then <m>y^2+y+1=0</m>, and the solutions to this are
        <me>
          x^2=y=\frac{1\pm \sqrt{5}}{2}
        </me>
      </p>
      <p>
        Thus, we see that <m>x=\pm \sqrt{\frac{1+\sqrt{5}}{2}}</m> are two solutions,
        we just need to find the other two.
        They will be solutions to <m>x^2 = \frac{1-\sqrt{5}}{2} = - \frac{\sqrt{5}-1}{2}</m>,
        which are <m>\pm i \sqrt{\frac{\sqrt{5}-1}{2}}</m>.
        Thus, all 4 solutions are
        <me>
          \pm \sqrt{\frac{1+\sqrt{5}}{2}}, \;\; \pm i \sqrt{\frac{\sqrt{5}-1}{2}}
        </me>.
      </p>
    </solution>
    <p>
      (c) <m>2x^4-4x^3+3x^2+2x-2</m>,
      given that one of the roots is <m>1+i</m>.
    </p>
    <solution>
      <p>
        Since this is a real polynomial,
        the conjugate of <m>1+i</m> is also a root,
        so two of the root are <m>1\pm i</m>.
        Hence, the polynomial contains
        <me>
          (x-(1+i))(x-(1-i))= x^2-2x+2
        </me>
        as a factor.
        Now let's do polynomial long division to find the other factor.
        The leading factor of our original polynomial is <m>2x^{4}</m>,
        which we can eliminate by subtracting <m>2x^2(x^2-2x+2)</m> to get
        <me>
          -x^2+2x-2=-(x^2-2x+2)
        </me>
      </p>
      <p>
        Then finally we can just subtract <m>-1\cdot (x^2-2x+2)</m> to eliminate this.
        Thus, we can factor the above polynomial as
        <me>
          2x^4-4x^3+3x^2+2x-2=(2x^2-1)(x^2-2x+2)=2(x-2^{-1/2})(x+2^{1/2})(x-(1+i))(x+(1-i))
        </me>
        so the roots are finally <m>\pm 2^{-1/2}, 1\pm i</m>.
      </p>
    </solution>
  </exercise>
  <exercise>
    <statement>
      <p>
        Factor the following polynomials into products of real polynomials that are linear and/or quadratic:
        <ul>
          <li>
            <p>
              <m>x^3-1</m>.
              <solution>
                <p>
                  We first need to find the roots of unity of <m>x^3</m>,
                  which are
                  <m>1,
                  w=e^{2\pi i/3}=-\frac{1}{2}+\sqrt{3}{2}i</m> and <m>w^2=e^{4\pi i/3} = -\frac{1}{2}-\sqrt{3}{2}i=\overline{w}</m>.
                  Thus,
                  <md>
                    <mrow>x^3-1 \amp  = (x-1)(x-w)(x-\overline{w}) = (x-1)(x^2-wx-\overline{w}x+\overline{w}w)</mrow>
                    <mrow>\amp  = (x-1)(x^2+x+|w|^2) = (x-1)(x^2+x+1)</mrow>
                  </md>.
                </p>
              </solution>
            </p>
          </li>
          <li>
            <p>
              <m>x^3+1</m>.
              <solution>
                <p>
                  We need to find the roots of <m>x^3+1=0</m>,
                  which are solutions to <m>x^3=-1=e^{\pi i}</m>.
                  One solution is clearly <m>1</m>.
                  Another we can get by taking 1/3 the exponent of <m>e^{\pi i}</m>,
                  which is <m>w=e^{\pi i/3} = \frac{1}{2}+\frac{\sqrt{3}}{2}</m>.
                  We know that roots of real polynomials come in conjugate pairs,
                  and so the other root is <m>\overline{w}</m>.
                  Thus,
                  <md>
                    <mrow>x^3+1 \amp  = (x-(-1))(x-w)(x-\overline{w}) = (x+1)(x^2-wx-\overline{w}x+\overline{w}w)</mrow>
                    <mrow>\amp  = (x+1)(x^2-x+|w|^2) = (x+1)(x^2-x+1)</mrow>
                  </md>.
                </p>
              </solution>
            </p>
          </li>
          <li>
            <p>
              <m>x^4-1</m>.
              <solution>
                <p>
                  There is no need to find complex roots here:
                  <me>
                    x^4-1 = (x^2)^2-1 = (x^2-1)(x^2+1)
                  </me>.
                </p>
              </solution>
            </p>
          </li>
          <li>
            <p>
              <m>x^4+1</m>.
              <solution>
                <p>
                  To find the roots of <m>x^4+1</m>,
                  we need to find solutions to <m>x^4=-1=e^{\pi i}</m>.
                  One solution is <m>z=e^{\pi i/4}=\frac{1}{\sqrt{2}}+\frac{1}{\sqrt{2}}i</m>.
                  To find all 4 roots, we just multiply this by the 4th roots of unity,
                  which are <m>\pm 1, \pm 1</m>,
                  thus all solutions which will be
                  <me>
                    \pm \frac{1}{\sqrt{2}} \pm \frac{1}{\sqrt{2}}i
                  </me>
                  where we consider all 4 possible combinations of <m>+</m>'s and <m>-</m>'s.
                  Let <m>z=\frac{1}{\sqrt{2}}+i\frac{1}{sqrt{2}}</m> and <m>w=-\frac{1}{\sqrt{2}}+i\frac{1}{\sqrt{2}}</m>.
                  Then the roots are <m>z,w,\overline{z},\overline{w}</m>.
                  Thus,
                  <md>
                    <mrow>x^4+1 \amp = (x-z)(z-\overline{z})(x-w)(x-\overline{w})</mrow>
                    <mrow>\amp  =(x^2 -zx-\overline{z}x+z\overline{z})(x^2 -wx-\overline{w}x+w\overline{w})</mrow>
                    <mrow>\amp  = (x^2-\sqrt{2}x+|z|^2)(x^2+\sqrt{2}x+|w|^2)</mrow>
                    <mrow>\amp  = (x^2-\sqrt{2}x+1)(x^2+\sqrt{2}x+1)</mrow>
                  </md>.
                </p>
              </solution>
            </p>
          </li>
          <li>
            <p>
              <m>x^5+1</m>.
              <term>Hint: <m>\cos \frac{2\pi}{5}= \frac{-1+\sqrt{5}}{4}</m> and <m>\cos \frac{4\pi}{5}= \frac{-1-\sqrt{5}}{4}</m>.</term>
              <solution>
                <p>
                  We note that this is easily completely factorized over the complex numbers.
                  Let <m>\xi = e^{\frac{2\pi i}{10}}</m>,
                  then the <m>5</m>th roots of unity are <m>1,\xi,\xi^2, \xi^3,\xi^4</m>.
                  By examining these numbers,
                  we can see that <m>\xi^{4}=\overline{\xi}</m> and <m>\xi^{3} = \overline{\xi}^{2}</m>.
                  Thus,
                  <me>
                    x^5+1 = (x+1)\underbrace{(x-\xi)(x-\bar{\xi})}_{\textrm{conjugate} }\underbrace{(x-\xi^2)(x-\bar{\xi}^2)}_{\textrm{conjugate} }
                  </me>.
                </p>
                <p>
                  If we collect into pairs the terms which involve a root and its conjugate,
                  we obtain real polynomials.
                </p>
                <p>
                  We compute:
                  <me>
                    (x-\xi)(x-\bar{\xi}) = x^2 - (\xi+\bar{\xi})x + \xi\bar{\xi} = x^2 - 2\cos(\frac{2\pi}{5})x+1 = x^2 +\frac{1-\sqrt{5}}{2}x+1
                  </me>.
                  and
                  <me>
                    (x-\xi^2)(x-\bar{\xi}^2) = x^2 -(\xi^2 + \bar{\xi}^2)x + \xi^2\bar{\xi}^2 = x^2 - 2\cos(\frac{4\pi}{5})x+1 = x^2 +\frac{1+\sqrt{5}}{2}x+1.
                  </me>,
                </p>
                <p>
                  Hence,
                  <me>
                    x^5 = \left(x^2 +\frac{1-\sqrt{5}}{2}x+1\right) \left(x^2 +\frac{1+\sqrt{5}}{2}x+1\right)
                  </me>.
                </p>
              </solution>
            </p>
          </li>
        </ul>
      </p>
    </statement>
  </exercise>
  <exercise>
    <statement>
      <p>
        If <m>x^3+15x^2+74x+120</m> has roots of the form <m>a,a+1,a+2</m>,
        find <m>a</m>.
      </p>
    </statement>
    <solution>
      <p>
        We see that by the Root-Coefficient Theorem,
        <me>
          -15=a+a+1+a+2=3a+3
        </me>
        and so <m>a=-6</m>.
      </p>
    </solution>
  </exercise>
  <exercise>
    <statement>
      <p>
        Let <m>a\in \mathbb{R}</m>.
        If <m>x^{3}-x+a</m> has three integer roots, solve for <m>a</m>.
      </p>
    </statement>
    <solution>
      <p>
        Note that if the integer roots are <m>r_{1},r_{2}</m>,
        and <m>r_{3}</m>, then by Proposition 7.1,
        <me>
          r_{1}+r_{2}+r_{3}=0
        </me>
        and
        <me>
          r_{1}r_{2}+r_{2}r_{3}+r_{3}r_{1}=-1
        </me>
      </p>
      <p>
        Hence,
        <me>
          r_{1}^{2}+r_{2}^{2}+r_{3}^{2} = (r_{1}+r_{2}+r_{3})^{2}-2(r_{1}r_{2}+r_{2}r_{3}+r_{3}r_{1})=2
        </me>.
      </p>
      <p>
        Since the <m>r_{i}</m> are integers,
        the <m>r_{i}^{2}</m> are nonnegative integers,
        and so one of them has to be zero.
        Thus, <m>0=0^{2}-0+a</m>, hence <m>a=0</m>.
      </p>
    </solution>
  </exercise>
  <exercise>
    <statement>
      <p>
        Show that if <m>z_1,z_2,z_3\in \C</m> are so that <m>z_1+z_2+z_3=0</m>,
        and <m>z_1^2+z_2^2+z_3^2=0</m> then <m>|z_1|=|z_2|=|z_3|</m>
      </p>
    </statement>
    <solution>
      <p>
        Let <m>f(z)=(z-z_1)(z-z_2)(z-z_3)</m>.
        Then <m>f(z)=z^3-az^2+bz-c</m> where
        <md>
          <mrow>a\amp =z_1+z_2+z_3</mrow>
          <mrow>b\amp =z_1z_2+z_2z_3+z_3z_1</mrow>
          <mrow>c\amp =z_1z_2z_3</mrow>
        </md>
      </p>
      <p>
        By assumption, we get that <m>a=z_1+z_2+z_3=0</m>.
        Also, since <m>z_{1}^2+z_{2}^2+z_{3}^2=0</m>, we have
        <me>
          (z_1+z_2+z_3)^2=z_1^2+z_2^2+z_3^2+2(z_1z_2+z_2z_3+z_3z_1)
        </me>
        and so <m>b=0</m>.
        Thus, <m>f(z)=z^3-c</m>, so in particular,
        since <m>z_{1},z_{2}</m> and <m>z_{3}</m> are roots,
        we have <m>z_{1}^3=z_{2}^3=z_{3}^{3}=c</m>.
        Thus
        <me>
          |c|=|z_{i}^3|=|z_{i}|^3
        </me>
        so <m>|z_{i}|=|c|^{1/3}</m> for <m>i=1,2,3</m>.
      </p>
    </solution>
  </exercise>
  <exercise>
    <statement>
      <p>
        Suppose <m>|z_{1}|=|z_{2}|=|z_{3}|=1</m> and <m>z_{1}+z_{2}+z_{3}=0</m>.
        Show that <m>z_{1}^3=z_{2}^3=z_{3}^3</m>.
        <term>Hint: First think about when <m>z_{1}=1</m>,
        then use that to prove the general case.</term>
      </p>
    </statement>
    <solution>
      <p>
        First let's assume <m>z_{1}=1</m>.
        Then <m>z_{2}+z_{3}=-1</m>.
        In particular,
        this means that the imaginary parts of <m>z_{2}</m> and <m>z_{3}</m> cancel, that is,
        if <m>z_{j}=x_{j}+iy_{j}</m>, then <m>y_{2}=-y_{3}</m>.
        Also, <m>x_{2}+x_{3}=-1</m>,
        and we can't have <m>x_{2}>0</m>,
        since then <m>x_{2}+x_{3}>x_{3}\geq -1</m>.
        Similarly, we can't have <m>x_{3}>0</m>,
        thus <m>x_{2},x_{3}\leq 0</m>.
        Also,
        <me>
          -x_{2} = \sqrt{1-y_{2}^2} = \sqrt{1-y_{3}^2}= -x_{3}
        </me>,
        hence <m>z_{3} = -x_{2} -iy_{2} = \overline{z_{2}}</m>,
        and <m>-1=z_{2}+z_{3}=-x_{2}-x_{2}=-2x_{2}</m>,
        thus <m>x_{2}=-\frac{1}{2}</m>.
        Thus, we must have that <m>z_{3} = -\frac{1}{2}\pm i\frac{\sqrt{3}}{2}</m>.
      </p>
      <p>
        For the general case, let <m>w_{i}=\overline{z_{1}}z_{i}</m>,
        then <m>w_{1}=1</m> and <m>w_{1}+w_{2}+w_{3}=0</m>.
        We now apply the previous case to conclude that
        <m>w_{i} = w^{i}</m> where <m>w=e^{2\pi i/3}</m>.
        Thus,
        <me>
          z_{j}^3 = (z_{1} w_{j})^3 = z_{1}^3 w_{j}^3 = z_{1} (w^{3j})=z_{1}
        </me>.
      </p>
    </solution>
  </exercise>
  <exercise>
    <statement>
      <p>
        Suppose <m>|z_{1}|=|z_{2}|=|z_{3}|=1</m> and <m>z_{1}+z_{2}+z_{3}=0</m>.
        Show that <m>z_{1}^{2^{n}}+z_{2}^{2^{n}}+z_{3}^{2^{n}}=0</m> for all <m>n\in \mathbb{N}</m>.
      </p>
    </statement>
    <solution>
      <p>
        By the previous problem,
        <m>z_1,z_2,z_3</m> are roots of <m>z^3-c</m> for some complex number <m>c</m> with <m>|c|=1</m>.
        In particular, by the Root-Coefficient Theorem,
        <me>
          z_{1}z_{2}+z_{1}z_{2}+z_{2}z_{3}=0
        </me>.
      </p>
      <p>
        Thus,
        <me>
          0=(z_{1}+z_{2}+z_{3})^2 = z_{1}^2+z_{2}^2+z_{3}^2 + 2(z_{1}z_{2}+z_{1}z_{2}+z_{2}z_{3})=z_{1}^2+z_{2}^2+z_{3}^2
        </me>.
      </p>
      <p>
        Now we can repeat the process by induction using
        <m>z_{1}^2,z_{2}^2,z_{3}^2</m> instead of <m>z_1,z_2,z_3</m>.
      </p>
    </solution>
  </exercise>
</section>