<section xml:id="proofbycontradiction">
  <title>Proof by Contradiction</title>
  <p>
    Suppose we have a statement <m>A</m> that we suspect is false.
    How can we prove that?
    One approach is to leverage a statement <m>B</m> that we
    <term>know</term> is false,
    and try to prove that <m>A \implies B</m>.
    Remember, <m>A \implies B</m> is the same thing as <m>\overline{A} \vee B</m>,
    so if we know that <m>B</m> is false,
    then the only alternative is that <m>A</m> is false.
    This is called proof by contradiction.
  </p>
  <theorem>
    <statement>
      <p>
        Let <m>A</m> and <m>B</m> be statements.
        Then <m>\overline{A \vee B}</m> is equivalent to <m>\overline{A} \wedge \overline{B}</m>.
      </p>
    </statement>
  </theorem>
  <proof>
    <p>
      We begin with the forward direction;
      that is, we shall show first that if <m>\overline{A \vee B}</m>,
      then <m>\overline{A} \wedge \overline{B}</m>.
      So let us assume <m>\overline{A \vee B}</m>.
      We aim to prove that both <m>\overline{A}</m> and <m>\overline{B}</m>.
    </p>
    <p>
      In other words,
      we need to show that <m>A</m> is <term>false</term>.
      So we want to prove that <m>A</m> implies something we know to be false.
      In our case, we are assuming that <m>\overline{A \vee B}</m>,
      so we know <m>A \vee B</m> to be false.
      This is great news: if <m>A</m> is true,
      then certainly <m>A \vee B</m> is true.
      That is, <m>A \implies (A \vee B)</m>.
      Since we know that <m>A \vee B</m> is false,
      that implies that <m>A</m> is false as well.
      Thus <m>\overline{A}</m> holds.
      Similarly, <m>B \implies (A \vee B)</m>,
      but that contradicts our assumption that <m>\overline{A \vee B}</m> is true.
      Thus <m>\overline{B}</m> holds.
    </p>
    <p>
      Now let's reverse directions;
      that is, let's show that if <m>\overline{A} \wedge \overline{B}</m>,
      then <m>\overline{A \vee B}</m>.
      So let us assume that both
      <m>\overline{A}</m> and <m>\overline{B}</m>.
      We aim to prove that <m>\overline{A \vee B}</m>.
    </p>
    <p>
      In other words, we need to show that
      <m>A \vee B</m> is <term>false</term>.
      If <m>A \vee B</m>, there are two options:
      <ul>
        <li>
          <p>
            One possibility is that <m>A</m> is true.
            But this would contradict our assumption that <m>\overline{A}</m> is true.
          </p>
        </li>
        <li>
          <p>
            So that leaves the other possibility,
            which is that <m>B</m> is true.
            But that contradicts our other assumption,
            that <m>\overline{B}</m> is true.
          </p>
        </li>
      </ul>
    </p>
    <p>
      Either way, we arrive at a contradiction,
      and so <m>A\vee B</m> is indeed false.
    </p>
  </proof>
  <p>
    As a quick corollary of this, we deduce that
    <me>
      \overline{A \wedge B} \iff \overline{\overline{\overline{A}} \wedge \overline{\overline{B}}} \iff \overline{\overline{\overline{A} \vee \overline{B}}} \iff (\overline{A} \vee \overline{B})
    </me>.
  </p>
  <p>
    Here's another example of proof by contradiction.
  </p>
  <example>
    <statement>
      <p>
        Let's say we want to prove that <m>\sqrt{3}\lt 1+\sqrt{2}</m>.
      </p>
    </statement>
    <proof>
      <p>
        Let's prove this by contradiction:
        we assume instead that <m>\sqrt{3}\geq 1+\sqrt{2}</m>,
        and we aim to deduce something we know to be false.
        If we square both sides of the inequality we assumed, we obtain
        <me>
          3\geq (1+\sqrt{2})^2=1+2\sqrt{2}+2=3+\sqrt{2}>3
        </me>,
        which is definitely false.
        We have thus shown by contradiction that <m>\sqrt{3}\lt  1+\sqrt{2}</m>.
      </p>
    </proof>
  </example>
  <p>
    Why didn't we do the same computations but with the original inequality?
    If we assumed <m>\sqrt{3}\lt  1+\sqrt{2}</m>,
    then squaring both sides gives
    <me>
      3\lt  (1+\sqrt{2})^2=1+2\sqrt{2}+2=3+\sqrt{2}
    </me>
    which is certainly true, but this doesn't help us.
    We started by assuming the thing we wanted to prove and then deducing something we know to be true. if <m>A</m> is the statement
    <q><m>\sqrt{3}\lt  1+\sqrt{2}</m></q>
    and <m>B</m> is the statement
    <q><m>3\lt 3+\sqrt{2}</m>,</q>
    then what we just showed was <m>A\implies B</m>,
    but that can't help us conclude that <m>A</m> is true.
    In our proof of <m>A</m> by contradiction,
    we assumed first that <m>A</m> is <term>false</term>,
    and then we deduce the statement <m>C</m>:
    <q><m>3>3</m>,</q>
    which we know perfectly well is false.
    Since <m>C</m> is false,
    the implication <m>\overline{A} \implies C</m> ensures that
    <m>\overline{A}</m> has to be false as well;
    in other words, <m>A</m> is true.
  </p>
</section>