<section xml:id="pythagoreantriples">
  <title>Application: Pythagorean Triples*</title>
  <p>
    In this section we will classify all Pythagorean Triples, that is,
    all positive integer solutions to
    <me>
      x^2+y^2=z^2
    </me>.
  </p>
  <p>
    This is a bit more involved than other diophantine problems and harder to figure out on your own on a homework problem
    (so it is not required reading),
    but we'll give a proof here since it's a neat application of what we've learned and can test your knowledge of the material in this chapter.
  </p>
  <p>
    We narrow down the solutions in a few steps:
    <ul>
      <li>
        <p>
          If <m>x=0</m>,
          then we must have <m>y^2=z^2</m>, and so <m>y=\pm z</m>.
          Thus, we know all solutions if <m>x=0</m>,
          so let's assume <m>x> 0</m>.
          Similarly, we can assume <m>y,z> 0</m>.
        </p>
      </li>
      <li>
        <p>
          We can assume that <m>x,y</m> and <m>z</m> are coprime
          (that is, no two of them share a common factor other than <m>1</m>).
          To see this, suppose <m>d=\gcd(x,y)</m>.
          Then <m>a=x/d</m> and <m>b=y/d</m> are coprime, and then
          <me>
            z^2= x^2+y^2 = d^2(a^2+b^2)
          </me>.
          By <xref ref="t_abn">Theorem</xref>,
          <m>a^2+b^2=c^2</m> for some integer <m>c</m>,
          and so <m>z^2=d^2 c^2=(cd)^2</m>.
          Hence, <m>(x,y,z)=(da,db,dc)</m> for some other Pythagorean Triple <m>(a,b,c)</m> where <m>a</m> and <m>b</m> are coprime.
          Thus, if we find all solutions <m>(x,y,z)</m> where <m>x</m> and <m>y</m> are coprime,
          then all other solutions are multiples of these.
          A similar proof shows that all solutions will be multiples of solutions where <m>x</m> and <m>z</m> are coprime and where <m>y</m> and <m>z</m> are coprime.
        </p>
      </li>
      <li>
        <p>
          Thus, assume <m>x,y</m>,
          and <m>z</m> are coprime and positive solutions to <m>x^2+y^2=z^2</m>.
          Then either <m>x</m> or <m>y</m> is odd, assume it is <m>x</m>.
        </p>
      </li>
      <li>
        <p>
          We now claim <m>z+y</m> and <m>z-y</m> are coprime.
          Suppose not.
          Then there is a prime <m>q</m> that divides them both.
          But then
          <me>
            q\text{ divides } (z+y)-(z-y) = 2y,\;\; q\text{ divides }  (z+y)+(z-y) = 2z
          </me>.
          Since <m>y</m> and <m>z</m> are coprime, <m>q=2</m>.
          But then
          <me>
            2\text{ divides } (z-y)(z+y)=z^{2}-y^{2}=x^{2}
          </me>
          which implies <m>x</m> is even, a contradiction.
        </p>
      </li>
      <li>
        <p>
          Since <m>z\pm y</m> are coprime and <m>x^{2}=(z+y)(z-y)</m>,
          we know that <m>z+y=s^{2}</m> and
          <m>z-y=t^{2}</m> for some integers <m>s</m> and <m>t</m> by <xref ref="t_abn">Theorem</xref>.
          Hence,
          <me>
            z=\frac{z+y+z-y}{2} = \frac{s^{2}+t^{2}}{2}
          </me>
          Similarly, <m>y=\frac{s^{2}-t^{2}}{2}</m>, and finally,
          <me>
            x^{2} =(z-y)(z+y) = s^{2}t^{2}
          </me>.
          Thus, all positive coprime solutions with <m>x</m> odd are of the form
          <me>
            (x,y,z) = \left( st, \frac{s^2-t^2}{2}, \frac{s^{2}+t^{2}}{2}\right)
          </me>.
        </p>
      </li>
      <li>
        <p>
          Finally, we now recall that all solutions are multiples of these soluitions,
          thus all Pythagorean Triples are of the form
          <me>
            (x,y,z) = \left( as t, a\frac{s^2-t^2}{2}, a\frac{s^{2}+t^{2}}{2}\right)
          </me>
          where <m>a,s,t</m> are integers.
        </p>
      </li>
    </ul>
  </p>
</section>