<section xml:id="realexercises">
  <title>Exercises</title>
  <p>
    The relevant exercises in Liebeck's book are at the end of Chapter 2.
  </p>
  <exercise>
    <statement>
      <p>
        Prove <m>(-1)^2=1</m>.
      </p>
    </statement>
    <solution>
      <p>
        By <xref ref="p_0x_0">Proposition</xref> and [M3]:
        <me>
          (-1)^2=(-1)\cdot (-1) = 1\cdot 1=1
        </me>.
      </p>
    </solution>
  </exercise>
  <exercise>
    <statement>
      <p>
        Let <m>F=\{0,1\}</m>, and for <m>a,b\in F</m>,
        define <m>a\cdot b</m> and <m>a+b</m> to equal what they would under normal multiplication except that now we define <m>1+1=0</m>.
        Is this a field?
      </p>
    </statement>
    <solution>
      <p>
        Yes.
        One can prove all the field properties on a case by case basis:
        for example,
        one can show <m>a+(b+c)=(a+b)+c</m> by try all possible values for <m>a,b</m> and <m>c</m>.
      </p>
    </solution>
  </exercise>
  <exercise>
    <statement>
      <p>
        Prove <m>\sqrt{6}</m> is irrational.
      </p>
    </statement>
    <solution>
      <p>
        Suppose <m>\sqrt{6}=\frac{p}{q}</m> where <m>p,q>0</m> are integers with no common factor.
        Then
        <me>
          6=\frac{p^2}{q^2} \;\; \Longrightarrow \;\;  6q^2=p^2
        </me>.
      </p>
      <p>
        Note that <m>p</m> must be even,
        so <m>p=2k</m> for some integer <m>k</m>, thus
        <me>
          6q^2=p^2=4k^2  \;\; \Longrightarrow \;\;   3q^2=2k^2
        </me>.
      </p>
      <p>
        Now <m>q</m> must be divisible by <m>2</m>.
        Otherwise, <m>q=2j+1</m> for some <m>j</m>, and so
        <me>
          2k^2=3q^2=3(2j+1)^2=12j^2+12j+3
        </me>
        which is a contradiction since now we have an even number equal to an odd number.
        Hence, <m>q=2j</m> for some integer <m>j</m>.
        But now <m>p</m> and <m>q</m> are both even,
        which contradicts our assumption that they had no common factor.
      </p>
    </solution>
  </exercise>
  <exercise>
    <statement>
      <p>
        Is <m>\sqrt{1+\sqrt{2}}</m> rational?
        Can you write a more general statement based on your proof?
      </p>
    </statement>
    <solution>
      <p>
        No.
        Suppose it were, then so is<m>\sqrt{1+\sqrt{2}}^2=1+\sqrt{2}</m>,
        and hence so is <m>\sqrt{2}=1+\sqrt{2}-1</m>.
      </p>
      <p>
        A more general statement is that if <m>x</m> is irrational,
        then so is <m>\sqrt{x}</m>,
        since otherwise <m>\sqrt{x}^2=x</m> is rational, a contradiction.
      </p>
    </solution>
  </exercise>
  <exercise>
    <statement>
      <p>
        Suppose <m>a+b\sqrt{2}=c+d\sqrt{2}</m> where <m>a,b,c,d\in\mathbb{Q}</m>.
        Prove that <m>a=c</m> and <m>b=d</m>.
      </p>
    </statement>
    <solution>
      <p>
        Homework question.
      </p>
    </solution>
  </exercise>
  <exercise>
    <statement>
      <p>
        Let
        <me>
          \mathbb{Q}[\sqrt{2}] = \{a+b\sqrt{2}\; |\; a,b\in\mathbb{Q}\}
        </me>.
      </p>
      <p>
        Show that <m>\mathbb{Q}[\sqrt{2}]</m> is a field using the usual rules of addition and multiplication.
      </p>
    </statement>
    <solution>
      <p>
        The only difficult property to verify is (M4), so let's focus on this.
        Let <m>a+b\sqrt{2}\in \mathbb{Q}[\sqrt{2}]</m> where <m>a,b\in\mathbb{Q}</m>.
        Note that
        <me>
          (a+b\sqrt{2})(a-b\sqrt{2})=a^2-2b^2
        </me>.
      </p>
      <p>
        Note that since <m>2</m> is irrational,
        we cannot have <m>a^2-2b^2=0</m>.
        Thus,
        <me>
          (a+b\sqrt{2}) \frac{a-b\sqrt{2}}{a^2-2b^2}=1
        </me>
        and so we have
        <me>
          (a+b\sqrt{2})^{-1} =\frac{a-b\sqrt{2}}{a^2-2b^2} =\frac{a}{a^2-2b^2}-\frac{b}{a^2-2b^2}\sqrt{2} \in\mathbb{Q}[\sqrt{2}]
        </me>.
      </p>
      <p>
        Thus, we have verified (M4).
      </p>
    </solution>
  </exercise>
  <exercise>
    <statement>
      <p>
        Are there rational numbers <m>a</m> and <m>b</m> so that <m>a\sqrt{2}+b\sqrt{3}=\sqrt{6}</m>?
      </p>
    </statement>
    <solution>
      <p>
        No.
        Suppose there were.
        They would both have to be non-zero.
        Then
        <me>
          6=(a\sqrt{2}+b\sqrt{3})^2=2a^2+3b^2+12ab\sqrt{6}
        </me>
        and so <m>\sqrt{6} = (6-(2a^2+3b^2))/(12ab)</m>,
        which is a rational number, but by an earlier exercise,
        <m>\sqrt{6}</m> is not rational, which is a contradiction.
      </p>
    </solution>
  </exercise>
  <p>
    \part{Week 2: Inequalities and Induction}
  </p>
</section>