<section xml:id="roots">
  <title>Roots</title>
  <p>
    In this class we will be working a lot with roots of numbers like <m>\sqrt{2}</m>,
    but like <m>\sqrt{2}</m>, that they exist at all takes justification.
    This is given in the following proposition whose proof we postpone until Week 3.
    Recall that <m>y^n=y\cdot y\cdots y</m> with <m>n</m> <m>y</m>'s in the product.
  </p>
  <proposition xml:id="p_roots-exist">
    <statement>
      <p>
        Given <m>x>0</m> and <m>n\in\mathbb{N}</m>,
        there is a unique <m>y>0</m> so that <m>y^n=x</m>,
        and we write this number <m>y</m> as <m>y=x^{\frac{1}{n}}</m>.
      </p>
    </statement>
  </proposition>
  <p>
    We can define more generally any rational root:
    if <m>\frac{m}{n}>0</m> is rational and <m>x>0</m>, we define
    <men xml:id="e_x_m_n">
      x^{\frac{m}{n}} = \left(x^{\frac{1}{n}}\right)^{m}=\underbrace{x^{\frac{1}{n}}\cdots x^{\frac{1}{n}}}_{m\mbox{ times} }
    </men>.
  </p>
  <proposition>
    <statement>
      <p>
        Let <m>x>0</m> and <m>p,q\in \mathbb{Q}</m>.
        Then
        <ol label="labelalph">
          <li>
            <p>
              <m>x^{p}x^q=x^{p+q}</m>
            </p>
          </li>
          <li>
            <p>
              <m>(x^{p})^{q}=x^{pq}</m>
            </p>
          </li>
          <li>
            <p>
              <m>(xy)^{p}=x^p y^p</m>.
            </p>
          </li>
        </ol>
      </p>
    </statement>
  </proposition>
  <note>
    <title>Try special cases</title>
    <p>
      When given something to prove as above,
      it might not be clear how to get started,
      but you don't have to prove everything on the first try!
      Try first proving the statement in some easier cases,
      and then see if you can adjust your proof or even use your easy cases to prove the general case.
    </p>
  </note>
  <proof>
    <ol label="labelalph">
      <li>
        <p>
          First notice that this holds when <m>p</m> and <m>q</m> are integers,
          since then
          <me>
            x^{p+q}=\underbrace{x\cdot x\cdots x}_{\mbox{\(p+q\) times} } =\underbrace{x\cdot x\cdots x}_{\mbox{\(p\) times} }\cdot \underbrace{x\cdot x\cdots x}_{\mbox{\(q\) times} } = x^{p}x^{q}
          </me>.
          Now suppose <m>p=\frac{a}{b}</m> and
          <m>q=\frac{c}{d}</m> are two positive rationals and <m>x>0</m>.
          Then
          <md>
            <mrow>x^{p+q} \amp  =x^{\frac{a}{b}+\frac{c}{d}} =x^{\frac{ad+bc}{bd}} \stackrel{(2.4.1)}{=} \left(x^{\frac{1}{bd}}\right)^{ad+bc} =\left(x^{\frac{1}{bd}}\right)^{ad}\left(x^{\frac{1}{bd}}\right)^{bc} \stackrel{(2.4.1)}{=}x^{\frac{ad}{bd}}x^{\frac{bc}{bd}}=x^{\frac{a}{b}}x^{\frac{c}{d}}=x^{p}x^{q}</mrow>
          </md>
          where in the fourth equation we used the integer case we proved earlier.
        </p>
      </li>
      <li>
        <p>
          Let's first prove the slightly simpler case that
          <men xml:id="e_x_abd">
            \left(x^{\frac{a}{b}}\right)^{\frac{1}{d}}=x^{\frac{a}{b}\cdot\frac{1}{d}}
          </men>.
          By <xref ref="p_roots-exist">Proposition</xref>,
          for the right side to equal the <m>d</m>th root on the left,
          we need to show <m>(x^{\frac{a}{b}\frac{1}{d}})^{d} = x^{\frac{a}{b}}</m>:
          <me>
            \left(x^{\frac{a}{b}\frac{1}{d}}\right)^{d} =\left(x^{\frac{a}{bd}}\right)^{d} \stackrel{(2.4.1)}{=} \left(\left(x^{\frac{1}{bd}}\right)^{a}\right)^{d} =\left(x^{\frac{1}{bd}}\right)^{ad} \stackrel{(2.4.1)}{=}x^{\frac{ad}{bd}}=x^{\frac{a}{b}}
          </me>,
          and so <xref ref="e_x_abd"/> follows.
          Now we prove the full case:
          if <m>p=\frac{a}{b}</m> and <m>q=\frac{c}{d}</m>, then
          <me>
            (x^{p})^{q} = \left(x^{\frac{a}{b}}\right)^{\frac{c}{d}} \stackrel{(2.4.1)}{=}\left( \left(x^{\frac{a}{b}}\right)^{\frac{1}{d}}\right)^{c} \stackrel{(2.4.2)}{=}\left(x^{\frac{a}{bd}}\right)^{c} \stackrel{(2.4.1)}{=} x^{\frac{ac}{bd}}=x^{pq}
          </me>.
          This proves (b).
        </p>
      </li>
      <li>
        <p>
          Let's first consider trying to show <m>(xy)^{\frac{1}{b}}=x^{\frac{1}{b}}y^{\frac{1}{b}}</m>.
          By <xref ref="p_roots-exist">Proposition</xref>,
          we just need to show that <m>(x^{\frac{1}{b}}y^{\frac{1}{b}})^{b}=xy</m>.
          If we take <m>x^{\frac{1}{b}}y^{\frac{1}{b}}</m> times itself <m>b</m> times,
          and rearrange the terms so that all the
          <m>x^{\frac{1}{b}}</m>'s are on the left, we get
          <me>
            (x^{\frac{1}{b}}y^{\frac{1}{b}})^{b} =x^{\frac{1}{b}}y^{\frac{1}{b}}  x^{\frac{1}{b}}y^{\frac{1}{b}}  \cdots x^{\frac{1}{b}}y^{\frac{1}{b}} =\underbrace{x^{\frac{1}{b}}\cdots x^{\frac{1}{b}}}_{b\mbox{ times} }\underbrace{y^{\frac{1}{b}}\cdots y^{\frac{1}{b}}}_{b\mbox{ times} } =(x^{\frac{1}{b}})^{b}(y^{\frac{1}{b}})^{b}=x\cdot y
          </me>.
          Now let's try the general case: If <m>p=\frac{a}{b}</m>,
          then by the case we just proved:
          <me>
            (xy)^{\frac{a}{b}} \stackrel{(2.4.1)}{=} \left((xy)^{\frac{1}{b}}\right)^{a} =\left(x^{\frac{1}{b}}y^{\frac{1}{b}}\right)^{a}
          </me>
          Just as before, if we take
          <m>x^{\frac{1}{b}}y^{\frac{1}{b}}</m> times itself <m>a</m> times and then move all the
          <m>x^{\frac{1}{b}}</m>'s to the left, we get that the above is
          <me>
            =(x^{\frac{1}{b}})^{a}(y^{\frac{1}{b}})^{a} \stackrel{(2.4.1)}{=} x^{\frac{a}{b}}y^{\frac{a}{b}}=x^{p}y^{p}
          </me>.
        </p>
      </li>
    </ol>
  </proof>
</section>