<section>
  <title>Order of a permutation</title>
  <p>
    Recall that <m>S_{n}</m> has <m>n!</m> elements.
    In particular, this means that if we look at the sequence
    <m>f,f^{2},f^{3},..</m>., eventually this must repeat on itself
    (otherwise we would have infinitely many distinct permutations on <m>n</m> integers,
    whereas we know there are only <m>n!</m> many).
    In other words, if we have a deck of <m>n</m> cards,
    and we shuffle the cards according to some permutation <m>f</m>,
    then no matter how random the shuffle is,
    so long as we use the <term>same</term> shuffle <m>f</m>,
    eventually the cards will return to their original order.
  </p>
  <p>
    In this section we'll show how to compute how soon powers of a permutation repeat.
  </p>
  <definition>
    <statement>
      <p>
        Let <m>f</m> be a permutation in <m>\mathrm{S}_n</m>.
        The smallest positive integer <m>m</m> such that
        <me>
          f^m=\iota
        </me>
        is called the <term>order</term> of the permutation <m>f</m>.
      </p>
    </statement>
  </definition>
  <p>
    The order of a cycle of length <m>r</m> is just <m>r</m>,
    which we saw earlier.
    In a few steps we will show how to compute the order of a permutation in general.
  </p>
  <lemma>
    <statement>
      <p>
        Let <m>f\in\mathrm{S}_n</m> have order <m>m</m>.
        If <m>f^k=\iota</m> for some integer <m>k\in\mathbb{N}</m>,
        then <m>m</m> divides <m>k</m>.
      </p>
    </statement>
  </lemma>
  <proof>
    <p>
      If <m>m</m> is the order of
      <m>f\in\mathrm{S}_n</m> and <m>f^k=\iota</m>,
      then by definition of <m>m</m>, <m>m\leq k</m>.
      By the remainder theorem,
      there are <m>q\geq 0</m> and
      <m>0\leq r\lt m</m> so that <m>k=qm+r</m>, and so
      <me>
        f^{k} = f^{qm+r} = (f^{m})^{q} f^{r} = (\iota)^{q}f^{r} = \iota f^{r}= f^{r}
      </me>.
    </p>
    <p>
      Recall that <m>m</m> is the smallest positive integer for which <m>f^{m}=\iota</m>,
      but now we have <m>r\in \{0,1,...,m-1\}</m>
      (and so <m>r\lt m</m>)
      for which <m>f^{r}=\iota</m>.
      This is only possible if <m>r</m> is not positive, i.e. if <m>r=0</m>.
      Thus, <m>k=qm+0=qm</m> so <m>m|k</m>.
    </p>
  </proof>
  <lemma>
    <statement>
      <p>
        Let <m>f\in\mathrm{S}_n</m> and let <m>m</m> be its order.
        Write
        <me>
          f=\sigma_{1}\sigma_{2}\cdots\sigma_{s}
        </me>
        where <m>\sigma_{1},\ldots,\sigma_{s}</m> are disjoint cycles of lengths <m>r_{1},\ldots,r_{s}</m> respectively.
        Then
        <me>
          m=\mathrm{lcm}\big(r_{1},r_{2},\ldots,r_{s}\big)
        </me>,
        where \mathrm{lcm} stands for the<nbsp/>least common multiple, that is,
        the smallest positive integer that is divisible by
        <m>\sigma_{i}</m> for each <m>i=1,...,s</m>.
      </p>
    </statement>
  </lemma>
  <proof>
    <p>
      Recall that the order of a cycle is just its length,
      so we know that <m>\sigma_i^{r_i}=\iota</m>.
      Notice that if <m>d= \mathrm{lcm}\big(r_{1},r_{2},\ldots,r_{s}\big)</m>,
      then <m>r_i|d</m> for all <m>i</m>.
      Also recall that disjoint cycles commute,
      so we can split the following product:
      <me>
        f^{d} = (\sigma_{1}\sigma_{2}\cdots\sigma_{s})^{d} =\sigma_{1}^{d}\sigma_{2}^{d}\cdots \sigma_{s}^{d} =(\sigma_{1}^{r_{1}})^{d/r_{1}}(\sigma_{2}^{r_{2}})^{d/r_{2}}\cdots(\sigma_{s}^{r_{s}})^{d/r_{s}} = (\iota)^{d/r_{1}}(\iota)^{d/r_{2}}\cdots (\iota)^{d/r_{s}}=\iota
      </me>.
    </p>
    <p>
      By the previous lemma, this means <m>m|d</m>.
      However, note that since <m>m</m> is the order of <m>f</m>,
      <me>
        \iota = f^{m} = (\sigma_{1}\sigma_{2}\cdots\sigma_{s})^{m} =\sigma_{1}^{m}\sigma_{2}^{m}\cdots \sigma_{s}^{m}
      </me>
      and since these cycles are disjoint,
      we must have that <m>\sigma_{i}^{m}=\iota</m> for each <m>i</m>.
      By the previous lemma again, this means <m>r_i|m</m>
      (since <m>r_i</m> is the order of <m>\sigma_i</m>).
      By the definition of the least common multiple, this means <m>d|m</m>.
      Finally, <m>m|d</m> and <m>d|m</m>
      (and both being positive integers)
      imply <m>d=m</m>.
    </p>
  </proof>
  <p>
    Using this Lemma,
    you can now always compute <m>m</m> by finding the cycle decomposition.
  </p>
  <example>
    <statement>
      <p>
        The<nbsp/>order of the<nbsp/>permutation
        <me>
          \left(\begin{matrix}1 \amp  2 \amp  3 \amp  4 \amp  5 \amp  6 \amp  7 \amp  8\cr3 \amp  4 \amp  6 \amp  1 \amp  5 \amp  2 \amp  8 \amp  7\cr \end{matrix} \right) = \big(1\ 3\ 6\ 2\ 4\big)\big(7\ 8\big)\in\mathrm{S}_{8}
        </me>,
        is <m>\mathrm{lcm}(2, 5, 1)=\mathrm{lcm}(2, 5)=10</m>,
        while the order of
        <me>
          \left(\begin{matrix}1 \amp  2 \amp  3 \amp  4 \amp  5 \amp  6 \amp  7 \amp  8\cr5 \amp  6 \amp  7 \amp  8 \amp  1 \amp  2 \amp  3 \amp  4\cr \end{matrix} \right) =  (1 \; 5)(2 \; 6)(3\; 7)(4\; 8) \in\mathrm{S}_{8}
        </me>,
        is <m>\mathrm{lcm}(2,2,2,2)=2</m>.
      </p>
    </statement>
  </example>
</section>