<section xml:id="stronginduction">
  <title>Strong Mathematical Induction</title>
  <p>
    Sometimes it's not enough to know that <m>P(n)</m> is true in order to prove that <m>P(n+1)</m> is true;
    we might additionally need to use that some of the previous statements <m>P(k), P(k+1), \dots , P(n-1)</m> are true.
  </p>
  <definition>
    <title>Principle of Strong Mathematical Induction</title>
    <statement>
      <p>
        Let <m>k\in \mathbb{N}</m> and let <m>P(k),P(k+1),..</m>. be statements.
        Suppose that
        <ul>
          <li>
            <p>
              <m>P(k)</m> is true, (base case)
            </p>
          </li>
          <li>
            <p>
              for any integer <m>n\geqslant k</m>, statements
              <me>
                P(k),P(k+1),P(k+2),\ldots,P(n)\mbox{{\color{blue} (all taken together)}} \Longrightarrow P(n+1)
              </me>
              (induction step).
            </p>
          </li>
        </ul>
      </p>
      <p>
        Then <m>P(n)</m> is true for every positive integer <m>n\geqslant k</m>.
      </p>
    </statement>
  </definition>
  <p>
    Strong induction is needed when you need to make use of several previous statements to prove the next one.
    For example:
  </p>
  <theorem>
    <statement>
      <p>
        Every integer <m>n\geq 2</m> can be written as a product of primes <m>n=p_{1}\cdots p_{k}</m>.
      </p>
    </statement>
  </theorem>
  <p>
    If <m>n</m> is prime, this statement still makes sense:
    we just interpret <m>n</m> as being the product of just one number,
    <m>n</m> itself.
  </p>
  <proof>
    <p>
      We prove by strong induction on <m>n</m>.
      The case <m>n=2</m> immediately holds
      (taking into account the previous remark).
      For the induction step,
      suppose the theorem holds for all integers <m>n\lt N</m>
      (this is our strong inductive hypothesis).
      If <m>N</m> is prime, there is nothing to prove;
      otherwise, if <m>N</m> is not prime,
      then <m>N=a\cdot b</m> for some positive integers <m>a</m> and <m>b</m> greater than <m>1</m>.
      Both <m>a</m> and <m>b</m> can be decomposed by the strong induction hypothesis,
      thus so can <m>n=ab</m>.
    </p>
  </proof>
  <p>
    Another situation when you need strong induction is when studying recurrence relations.
    A <term>recurrence</term> relation is a sequence
    <m>a_{1},a_{2},..</m>. of numbers where each <m>a_{n}</m> is defined in terms of previous terms in the sequence.
    The most famous recurrence relation is the
    <term>Fibonacci sequence</term>,
    which is defined as <m>f_{1}=1</m>,
    <m>f_{2}=1</m> and for <m>n>2</m>,
    <m>f_{n}=f_{n-1}+f_{n-2}</m>.
  </p>
  <example>
    <statement>
      <p>
        Let <m>x_{1}=1, x_{2} =3</m> and for <m>n\geq 2</m>, let
        <me>
          x_{n+1} = 4x_{n}-3x_{n-1}
        </me>.
      </p>
      <p>
        Let's try and find a general pattern for what <m>x_{n}</m> is.
        If we test the first few values, we get
        <me>
          x_{1} = 1, \;\; x_{2} = 3 , \;\; x_{3} = 4\cdot 3-3\cdot 1 = 9, \;\; x_{4} = 4\cdot 9 - 3\cdot 3 = 27
        </me>
        so it seems like <m>x_{n} = 3^{n-1}</m>.
        We will prove this by strong induction.
        Let <m>P(n)</m> be the statement
        <q><m>x_{n} = 3^{n-1}</m>.</q>
        Let's first prove the first two base cases:
        <m>x_{1}=1=3^{1-1}</m> and <m>x_{2}=3=3^{2-1}</m>,
        so <m>P(1)</m> and <m>P(2)</m> are true.
        Now suppose <m>P(k)</m> is true for
        <m>k=1,2,...,n</m> for some <m>n\geq 2</m>.
        Then
        <me>
          x_{n+1} =4x_{n}-3x_{n-1} = 4\cdot 3^{n-1} -3x_{n-1} = 4\cdot 3^{n-1} - 3\cdot 3^{n-2} = 3^{n} = 3^{(n+1)-1}
        </me>.
      </p>
      <p>
        This proves the induction step,
        and thus <m>x_n=3^{n-1}</m> for all <m>n</m> by strong induction.
      </p>
      <p>
        <em>Discussion:</em> <term>Why did we prove two base cases?</term>
        Note that the formula <m>x_{n+1} =4x_{n}-3x_{n-1}</m> holds only for <m>n\geq 2</m>,
        so in particular, I can't use it to prove <m>P(2)</m> (i.e. that <m>x_{2}=3^{2-1}</m>).
        For this reason, I need to prove a few more base cases that can't be covered in my induction step.
      </p>
      <p>
        <term>Why did we need strong induction instead of induction?</term>
        I needed both <m>P(n)</m> and <m>P(n-1)</m> to be true to prove <m>P(n+1)</m>,
        but with standard induction I would need to prove <m>P(n+1)</m> follows from just <m>P(n)</m>.
      </p>
    </statement>
  </example>
  <note>
    <p>
      <term>How do I know when to use induction vs. strong induction?</term>
      One way is to first try proving the induction step to see how many previous cases you need,
      then that will tell you how many base cases you need as well:
      if it is more than one, then you need strong induction.
    </p>
  </note>
</section>