<section xml:id="summationnotation">
  <title>Preliminaries on <m>\Sigma</m> notation</title>
  <p>
    Before getting into induction,
    it will be useful to review <m>\Sigma</m> notation.
    <m>\Sigma</m> notation is spoken as
    <q>sigma notation</q>
    after the Greek letter <m>\Sigma</m>.
  </p>
  <definition>
    <statement>
      <p>
        Given a sequence of numbers <m>a_{m},a_{m+1},...,a_{n}</m>, we write
        <me>
          \sum_{k=m}^{n} a_{k} = a_{m}+a_{m+1}+\cdots +a_{n}
        </me>.
      </p>
    </statement>
  </definition>
  <p>
    For example,
    <me>
      \sum_{k=1}^{n} k^2 = 1^2+2^2+3^2+\cdots + n^2
    </me>.
  </p>
  <p>
    We can split sums and use the distribution
    <me>
      \sum_{k=m}^{n} (a_{k} +b_{k})=\sum_{k=m}^{n} a_{k} +\sum_{k=m}^{n} b_{k}\;\; \;\;\; \mbox{ and } \;\;\;\;\; \sum_{k=m}^{n} c\cdot a_{k} =c\cdot \sum_{k=m}^{n} a_{k}
    </me>.
  </p>
  <p>
    <em>Note:</em> this is why we sometimes call numbers <term>constants</term>:
    the number <m>c</m> when it appears inside a sum does not vary as <m>k</m> changes,
    and for this reason we can factor it outside the sum.
  </p>
  <p>
    The following are useful manipulations of <m>\Sigma</m> notation
    <ol>
      <li>
        <p>
          Detaching the last element:
          <me>
            \sum_{k=1}^{n+1} a_k = \left(\sum_{k=1}^{n} a_k\right) + a_{n+1}
          </me>.
        </p>
      </li>
      <li>
        <p>
          Differences
          <me>
            \mbox{If }  S_n=\sum_{k=1}^{n} a_k, \mbox{ then }  S_{n+1}-S_n = a_{n+1}
          </me>.
        </p>
      </li>
      <li>
        <p>
          Change of variables:
          <me>
            \sum_{k=m}^{n} a_{k+\ell} =\sum_{k=m+\ell}^{n+\ell} a_{k}
          </me>.
          For example,
          <me>
            \sum_{k=3}^{5} \frac{1}{(k+1)^2} =\frac{1}{(3+1)^2}+\frac{1}{(4+1)^2}+\frac{1}{(5+1)^2} =\frac{1}{4^2}+\frac{1}{5^2}+\frac{1}{6^2} = \sum_{k=4}^{6} \frac{1}{k^2}
          </me>.
        </p>
      </li>
      <li>
        <p>
          Change of variables:
          <me>
            \sum_{k=m}^{n} a_{k} =\sum_{j=m}^{n} a_{j}
          </me>.
        </p>
      </li>
    </ol>
  </p>
</section>